cedar-lean/Cedar/Thm/PartialEval/Binary.lean
@@ -1,0 +1,182 @@
+/-
+ Copyright 2022-2023 Amazon.com, Inc. or its affiliates. All Rights Reserved.
+
+ Licensed under the Apache License, Version 2.0 (the "License");
+ you may not use this file except in compliance with the License.
+ You may obtain a copy of the License at
+
+      https://www.apache.org/licenses/LICENSE-2.0
+
+ Unless required by applicable law or agreed to in writing, software
+ distributed under the License is distributed on an "AS IS" BASIS,
+ WITHOUT WARRANTIES OR CONDITIONS OF ANY KIND, either express or implied.
+ See the License for the specific language governing permissions and
+ limitations under the License.
+-/
+
+import Cedar.Spec.PartialEvaluator
+import Cedar.Spec.Policy
+import Cedar.Thm.Data.Control
+import Cedar.Thm.Data.Map
+import Cedar.Thm.Data.Set
+import Cedar.Thm.PartialEval.Basic
+
+namespace Cedar.Thm.PartialEval.Binary
+
+open Cedar.Data
+open Cedar.Spec
+open Except
+
+/--
+  helper lemma: any subexpression of x₁ is a subexpression of (x₁ op x₂)
+-/
+theorem lhs_subexpression {x₁ x₂ x : PartialExpr} {op : BinaryOp} :
+  x ∈ x₁.subexpressions → x ∈ (PartialExpr.binaryApp op x₁ x₂).subexpressions
+:= by
+  intro h₁
+  unfold PartialExpr.subexpressions
+  simp [List.append_eq_append]
+  right ; left ; assumption
+
+/--
+  helper lemma: any subexpression of x₂ is a subexpression of (x₁ op x₂)
+-/
+theorem rhs_subexpression {x₁ x₂ x : PartialExpr} {op : BinaryOp} :
+  x ∈ x₂.subexpressions → x ∈ (PartialExpr.binaryApp op x₁ x₂).subexpressions
+:= by
+  intro h₁
+  unfold PartialExpr.subexpressions
+  simp [List.append_eq_append]
+  right ; right ; assumption
+
+/--
+  helper lemma: if LHS of a `PartialExpr.binaryApp` contains an unknown, the whole expression does
+-/
+theorem lhs_unknown {x₁ x₂ : PartialExpr} {op : BinaryOp} :
+  x₁.containsUnknown → (PartialExpr.binaryApp op x₁ x₂).containsUnknown
+:= by
+  unfold PartialExpr.containsUnknown
+  repeat rw [List.any_eq_true]
+  intro h₁
+  replace ⟨subx, h₁⟩ := h₁
+  exists subx
+  constructor
+  case left => apply lhs_subexpression h₁.left
+  case right => exact h₁.right
+
+/--
+  helper lemma: if RHS of a `PartialExpr.binaryApp` contains an unknown, the whole expression does
+-/
+theorem rhs_unknown {x₁ x₂ : PartialExpr} {op : BinaryOp} :
+  x₂.containsUnknown → (PartialExpr.binaryApp op x₁ x₂).containsUnknown
+:= by
+  unfold PartialExpr.containsUnknown
+  repeat rw [List.any_eq_true]
+  intro h₁
+  replace ⟨subx, h₁⟩ := h₁
+  exists subx
+  constructor
+  case left => apply rhs_subexpression h₁.left
+  case right => exact h₁.right
+
+/--
+  `PartialEntities.ancestorsOrEmpty` on concrete entities is the same as `Entities.ancestorsOrEmpty` on those entities
+-/
+theorem partial_ancestorsOrEmpty_on_concrete_eqv_ancestorsOrEmpty {entities : Entities} {uid : EntityUID} :
+  PartialEntities.ancestorsOrEmpty entities uid = Entities.ancestorsOrEmpty entities uid
+:= by
+  unfold PartialEntities.ancestorsOrEmpty Entities.ancestorsOrEmpty
+  unfold Entities.asPartialEntities EntityData.asPartialEntityData
+  rw [← Map.find?_mapOnValues]
+  cases h₁ : entities.find? uid <;> simp
+
+/--
+  `partialInₑ` on concrete arguments is the same as `inₑ` on those arguments
+-/
+theorem partialInₑ_on_concrete_eqv_inₑ {uid₁ uid₂ : EntityUID} {entities : Entities} :
+  partialInₑ uid₁ uid₂ entities = inₑ uid₁ uid₂ entities
+:= by
+  unfold partialInₑ inₑ
+  cases uid₁ == uid₂ <;> simp
+  case false => simp [partial_ancestorsOrEmpty_on_concrete_eqv_ancestorsOrEmpty]
+
+/--
+  `partialInₛ` on concrete arguments is the same as `inₛ` on those arguments
+-/
+theorem partialInₛ_on_concrete_eqv_inₛ {uid : EntityUID} {vs : Set Value} {entities : Entities} :
+  partialInₛ uid vs entities = inₛ uid vs entities
+:= by
+  unfold partialInₛ inₛ
+  simp [partialInₑ_on_concrete_eqv_inₑ]
+
+/--
+  `partialApply₂` on concrete arguments is the same as `apply₂` on those arguments
+-/
+theorem partialApply_on_concrete_eqv_apply {op : BinaryOp} {v₁ v₂ : Value} {entities : Entities} :
+  partialApply₂ op v₁ v₂ entities = (apply₂ op v₁ v₂ entities).map PartialValue.value
+:= by
+  unfold partialApply₂ apply₂ Except.map
+  cases op <;> split <;> rename_i h <;> simp only [false_implies, forall_const] at h <;> try simp
+  case add | sub | mul => split <;> rename_i h <;> simp [h]
+  case mem.h_10 uid₁ uid₂ => simp [partialInₑ_on_concrete_eqv_inₑ]
+  case mem.h_11 uid vs =>
+    simp [partialInₛ_on_concrete_eqv_inₛ]
+    cases inₛ uid vs entities <;> simp only [bind_err, bind_ok]
+  case mem.h_12 =>
+    split <;> simp only [error.injEq] <;> rename_i h₂ <;> split at h₂ <;> try simp at *
+    assumption
+
+/--
+  Inductive argument that partial evaluating a concrete `PartialExpr.binaryApp`
+  expression gives the same output as concrete-evaluating the `Expr.binaryApp` with
+  the same subexpressions
+-/
+theorem partial_eval_on_concrete_eqv_concrete_eval {x₁ x₂ : Expr} {request : Request} {entities : Entities} {op : BinaryOp} :
+  partialEvaluate x₁ request entities = (evaluate x₁ request entities).map PartialValue.value →
+  partialEvaluate x₂ request entities = (evaluate x₂ request entities).map PartialValue.value →
+  partialEvaluate (PartialExpr.binaryApp op x₁ x₂) request entities = (evaluate (Expr.binaryApp op x₁ x₂) request entities).map PartialValue.value
+:= by
+  intro ih₁ ih₂
+  unfold partialEvaluate evaluate
+  simp [ih₁, ih₂]
+  simp [Except.map, pure, Except.pure, Result.as, Coe.coe, Lean.Internal.coeM, CoeT.coe, CoeHTCT.coe, CoeHTC.coe, CoeOTC.coe, CoeTC.coe]
+  split <;> simp
+  case h_1 e h₁ => simp [h₁]
+  case h_2 v₁ h₁ =>
+    simp [h₁]
+    split <;> simp
+    case h_1 e h₂ => simp [h₂]
+    case h_2 v₂ h₂ => simp [h₂, partialApply_on_concrete_eqv_apply, Except.map]
+
+/--
+  Inductive argument for `ResidualsContainUnknowns` for `PartialExpr.binaryApp`
+-/
+theorem residuals_contain_unknowns {x₁ x₂ : PartialExpr} {request : PartialRequest} {entities : PartialEntities} {op : BinaryOp} :
+  @ResidualsContainUnknowns x₁ request entities →
+  @ResidualsContainUnknowns x₂ request entities →
+  @ResidualsContainUnknowns (PartialExpr.binaryApp op x₁ x₂) request entities
+:= by
+  unfold ResidualsContainUnknowns
+  intro ih₁ ih₂ r h₁
+  unfold partialEvaluate at h₁
+  cases h₂ : (partialEvaluate x₁ request entities) <;> simp [h₂] at h₁
+  cases h₃ : (partialEvaluate x₂ request entities) <;> simp [h₃] at h₁
+  case ok.ok pval₁ pval₂ =>
+    cases pval₁ <;> cases pval₂ <;> simp at h₁
+    case value.value v₁ v₂ =>
+      simp [partialApply₂] at h₁
+      cases op <;> split at h₁ <;> rename_i h <;> simp at h <;> try simp at h₁
+      case add i j => cases h₄ : intOrErr (Int64.add? i j) <;> simp [h₄] at h₁
+      case sub i j => cases h₄ : intOrErr (Int64.sub? i j) <;> simp [h₄] at h₁
+      case mul i j => cases h₄ : intOrErr (Int64.mul? i j) <;> simp [h₄] at h₁
+      case mem uid vs => cases h₄ : partialInₛ uid vs entities <;> simp [h₄] at h₁
+    case residual.value r₁ v₂ | residual.residual r₁ r₂ =>
+      subst h₁
+      apply lhs_unknown
+      apply @ih₁ r₁ h₂
+    case value.residual v₁ r₂ =>
+      subst h₁
+      apply rhs_unknown
+      apply @ih₂ r₂ h₃
+
+end Cedar.Thm.PartialEval.Binary
