cedar-lean/Cedar/Thm/PartialEval/Ite.lean
@@ -1,0 +1,125 @@
+/-
+ Copyright 2022-2023 Amazon.com, Inc. or its affiliates. All Rights Reserved.
+
+ Licensed under the Apache License, Version 2.0 (the "License");
+ you may not use this file except in compliance with the License.
+ You may obtain a copy of the License at
+
+      https://www.apache.org/licenses/LICENSE-2.0
+
+ Unless required by applicable law or agreed to in writing, software
+ distributed under the License is distributed on an "AS IS" BASIS,
+ WITHOUT WARRANTIES OR CONDITIONS OF ANY KIND, either express or implied.
+ See the License for the specific language governing permissions and
+ limitations under the License.
+-/
+
+import Cedar.Spec.PartialEvaluator
+import Cedar.Spec.Policy
+import Cedar.Thm.Data.Control
+import Cedar.Thm.PartialEval.Basic
+
+namespace Cedar.Thm.PartialEval.Ite
+
+open Cedar.Spec
+open Except
+
+/--
+  helper lemma: any subexpression of x₁ is a subexpression of (if x₁ then x₂ else x₃)
+-/
+theorem guard_subexpression {x₁ x₂ x₃ x : PartialExpr} :
+  x ∈ x₁.subexpressions → x ∈ (PartialExpr.ite x₁ x₂ x₃).subexpressions
+:= by
+  intro h₁
+  unfold PartialExpr.subexpressions
+  simp [List.append_eq_append]
+  right ; left ; assumption
+
+/--
+  helper lemma: if guard of a `PartialExpr.ite` contains an unknown, the whole expression does
+-/
+theorem guard_unknown {x₁ x₂ x₃ : PartialExpr} :
+  x₁.containsUnknown → (PartialExpr.ite x₁ x₂ x₃).containsUnknown
+:= by
+  unfold PartialExpr.containsUnknown
+  repeat rw [List.any_eq_true]
+  intro h₁
+  replace ⟨subx, h₁⟩ := h₁
+  exists subx
+  constructor
+  case left => apply guard_subexpression h₁.left
+  case right => exact h₁.right
+
+/--
+  Inductive argument that partial evaluating a concrete `PartialExpr.ite`
+  expression gives the same output as concrete-evaluating the `Expr.ite` with
+  the same subexpressions
+-/
+theorem partial_eval_on_concrete_eqv_concrete_eval {x₁ x₂ x₃ : Expr} {request : Request} {entities : Entities} :
+  partialEvaluate x₁ request entities = (evaluate x₁ request entities).map PartialValue.value →
+  partialEvaluate x₂ request entities = (evaluate x₂ request entities).map PartialValue.value →
+  partialEvaluate x₃ request entities = (evaluate x₃ request entities).map PartialValue.value →
+  partialEvaluate (PartialExpr.ite x₁ x₂ x₃) request entities = (evaluate (Expr.ite x₁ x₂ x₃) request entities).map PartialValue.value
+:= by
+  intro ih₁ ih₂ ih₃
+  unfold partialEvaluate evaluate
+  simp [ih₁, ih₂, ih₃]
+  simp [Except.map, pure, Except.pure, Result.as, Coe.coe, Lean.Internal.coeM, CoeT.coe, CoeHTCT.coe, CoeHTC.coe, CoeOTC.coe, CoeTC.coe]
+  split <;> simp
+  case h_1 e h₁ => simp [h₁]
+  case h_2 v h₁ =>
+    simp [h₁, Value.asBool]
+    cases v <;> try simp only [bind_err]
+    case prim p =>
+      cases p <;> simp only [bind_ok, bind_err]
+      case bool b =>
+        cases b <;> simp only [ite_true, ite_false]
+
+/--
+  Inductive argument for `ResidualsContainUnknowns` for `PartialExpr.ite`
+-/
+theorem residuals_contain_unknowns {x₁ x₂ x₃ : PartialExpr} {request : PartialRequest} {entities : PartialEntities} :
+  @ResidualsContainUnknowns x₁ request entities →
+  @ResidualsContainUnknowns x₂ request entities →
+  @ResidualsContainUnknowns x₃ request entities →
+  @ResidualsContainUnknowns (PartialExpr.ite x₁ x₂ x₃) request entities
+:= by
+  unfold ResidualsContainUnknowns
+  intro ih₁ ih₂ ih₃ r h₁
+  unfold partialEvaluate at h₁
+  cases h₂ : (partialEvaluate x₁ request entities) <;> simp [h₂] at h₁
+  case ok pval₁ =>
+    cases pval₁ <;> simp at h₁
+    case residual r₁ =>
+      -- partial evaluating the guard produced a residual
+      subst h₁
+      apply guard_unknown
+      apply @ih₁ r₁ h₂
+    case value v₁ =>
+      -- partial evaluating the guard produced a value v₁
+      cases v₁ <;> simp [Value.asBool] at h₁
+      case prim p₁ =>
+        cases p₁
+        case int | string | entityUID => cases h₁
+        case bool b₁ =>
+          cases b₁ <;> simp at h₁
+          case false =>
+            -- partial evaluating the guard produced ok-false
+            cases h₃ : (partialEvaluate x₃ request entities) <;> simp [h₃] at h₁
+            case ok pval₂ =>
+              cases pval₂ <;> simp at h₁
+              case residual r₂ =>
+                -- partial evaluating the else-expr produced a residual
+                subst h₁
+                apply @ih₃ r₂ h₃
+          case true =>
+            -- partial evaluating the guard produced ok-true
+            cases h₃ : (partialEvaluate x₂ request entities) <;> simp [h₃] at h₁
+            case ok pval₂ =>
+              cases pval₂ <;> simp at h₁
+              case residual r₂ =>
+                -- partial evaluating the then-expr produced a residual
+                subst h₁
+                apply @ih₂ r₂ h₃
+
+end Cedar.Thm.PartialEval.Ite
