cedar-lean/Cedar/Thm/PartialEval/Unary.lean
@@ -1,0 +1,96 @@
+/-
+ Copyright 2022-2023 Amazon.com, Inc. or its affiliates. All Rights Reserved.
+
+ Licensed under the Apache License, Version 2.0 (the "License");
+ you may not use this file except in compliance with the License.
+ You may obtain a copy of the License at
+
+      https://www.apache.org/licenses/LICENSE-2.0
+
+ Unless required by applicable law or agreed to in writing, software
+ distributed under the License is distributed on an "AS IS" BASIS,
+ WITHOUT WARRANTIES OR CONDITIONS OF ANY KIND, either express or implied.
+ See the License for the specific language governing permissions and
+ limitations under the License.
+-/
+
+import Cedar.Spec.PartialEvaluator
+import Cedar.Spec.Policy
+import Cedar.Thm.Data.Control
+import Cedar.Thm.PartialEval.Basic
+
+namespace Cedar.Thm.PartialEval.Unary
+
+open Cedar.Spec
+open Except
+
+/--
+  helper lemma: any subexpression of x₁ is a subexpression of (unaryApp op x₁)
+-/
+theorem operand_subexpression {x₁ x : PartialExpr} {op : UnaryOp} :
+  x ∈ x₁.subexpressions → x ∈ (PartialExpr.unaryApp op x₁).subexpressions
+:= by
+  intro h₁
+  unfold PartialExpr.subexpressions
+  simp [List.append_eq_append]
+  right ; assumption
+
+/--
+  helper lemma: if the operand of a `unaryApp` contains an unknown, the whole
+  expression does
+-/
+theorem operand_unknown {x₁ : PartialExpr} {op : UnaryOp} :
+  x₁.containsUnknown → (PartialExpr.unaryApp op x₁).containsUnknown
+:= by
+  unfold PartialExpr.containsUnknown
+  repeat rw [List.any_eq_true]
+  intro h₁
+  replace ⟨subx, h₁⟩ := h₁
+  exists subx
+  constructor
+  case left => apply operand_subexpression h₁.left
+  case right => exact h₁.right
+
+/--
+  Inductive argument that partial evaluating a concrete `PartialExpr.unaryApp`
+  expression gives the same output as concrete-evaluating the `Expr.unaryApp` with
+  the same subexpressions
+-/
+theorem partial_eval_on_concrete_eqv_concrete_eval {x₁ : Expr} {request : Request} {entities : Entities} {op : UnaryOp} :
+  partialEvaluate x₁ request entities = (evaluate x₁ request entities).map PartialValue.value →
+  partialEvaluate (PartialExpr.unaryApp op x₁) request entities = (evaluate (Expr.unaryApp op x₁) request entities).map PartialValue.value
+:= by
+  intro ih₁
+  unfold partialEvaluate evaluate
+  simp [ih₁]
+  simp [Except.map, pure, Except.pure, Result.as, Coe.coe, Lean.Internal.coeM, CoeT.coe, CoeHTCT.coe, CoeHTC.coe, CoeOTC.coe, CoeTC.coe]
+  split <;> simp
+  case h_1 e h₁ => simp [h₁]
+  case h_2 v h₁ =>
+    simp [h₁]
+    split
+    case h_1 h₂ | h_2 h₂ => simp [h₂]
+
+/--
+  Inductive argument for `ResidualsContainUnknowns` for `PartialExpr.unaryApp`
+-/
+theorem residuals_contain_unknowns {x₁ : PartialExpr} {request : PartialRequest} {entities : PartialEntities} {op : UnaryOp} :
+  @ResidualsContainUnknowns x₁ request entities →
+  @ResidualsContainUnknowns (PartialExpr.unaryApp op x₁) request entities
+:= by
+  unfold ResidualsContainUnknowns
+  intro ih₁ r h₁
+  unfold partialEvaluate at h₁
+  cases h₂ : (partialEvaluate x₁ request entities) <;> simp [h₂] at h₁
+  case ok pval₁ =>
+    cases pval₁ <;> simp at h₁
+    case residual r₁ =>
+      -- partial evaluating the operand produced a residual
+      subst h₁
+      apply operand_unknown
+      apply @ih₁ r₁ h₂
+    case value v₁ =>
+      -- partial evaluating the operand produced a value v₁
+      cases h₃ : apply₁ op v₁ <;> simp [h₃] at h₁
+
+end Cedar.Thm.PartialEval.Unary
